Test/Common.lean
@@ -40,6 +40,7 @@ deriving instance DecidableEq, Repr for Expression
 deriving instance DecidableEq, Repr for Variable
 deriving instance DecidableEq, Repr for Goal
 deriving instance DecidableEq, Repr for InvokedTerm
+deriving instance DecidableEq, Repr for InvokedSyntaxArgument
 deriving instance DecidableEq, Repr for ExprEchoResult
 deriving instance DecidableEq, Repr for InteractionError
 deriving instance DecidableEq, Repr for Option
